% Consider the Fourier transformation $\mathcal{F}: L^2(\mathbb{R}^d)\to L^2(\mathbb{R}^d)$ and its inverse
% \begin{equation}
% \begin{split}
% \mathcal{F}f(\omega) &:= \frac{1}{(\sqrt{2\pi})^d}\int f(x) \zeta_\omega(x) \mathrm{d}x \\
% \hat{\mathcal{F}}\hat{f}(\omega) &:= \frac{1}{(\sqrt{2\pi})^d}\int \hat{f}(x) \zeta_\omega^{\ast}(x) \mathrm{d}\omega
% \end{split}
% \end{equation}
% where we write $\hat{f} := \mathcal{F}f$, $\zeta_\omega(x):=\exp(-\sqrt{-1}\omega^Tx)$ for short.

% \begin{theorem}
% For continuous even function $\psi: \mathbb{R}^d\to \mathbb{R}$, we define symmetric function $k: \mathbb{R}^d \times \mathbb{R}^d \to \mathbb{R}$ by $k(x, x') = \psi(x-x')$. $k$ is positive semi-definite if and only if the $\hat{\psi}$ is non-negative.
% \end{theorem}

Therefore if $k(x, x') = \psi(x-y)$ is positive semi-definite kernel,
if we can define the probability distribution $p(\omega)\propto \hat{\psi}(\omega)$.
We can define 
\begin{equation}
\begin{split}
k(x, x') &= \hat{\mathcal{F}} \hat{\psi}(x-x') \\
         &= \frac{1}{(\sqrt{2\pi})^d} \int \hat{\psi}(\omega) \zeta_\omega^{\ast}(x-x') \mathrm{d}\omega\\
         &= C \int p(\omega) \zeta_\omega^{\ast}(x) \zeta_\omega(x') \mathrm{d}\omega\\
         &= C \mathbb{E}_{\omega\sim p}\left[\zeta_\omega^{\ast}(x) \zeta_\omega(x')\right]
\end{split}
\end{equation}
where $C=\frac{1}{(\sqrt{2\pi})^d}\int \hat{\psi}(\omega)\mathrm{d}\omega$ is a normalizing constant.
As we can write the kernel value as an expectation of some probability,
we get the unbiased estimate of $k(x, x')$ by sampling $\omega$ from this distribution.
\begin{equation}
k(x, x') \approx \frac{C}{N} \sum_{n=1}^{N} \zeta_{\omega_n}^{\ast}(x) \zeta_{\omega_n}(x')
\end{equation}
where $\omega_n \sim p(\omega)$, i.i.d..

Consider the data distribution $\mathcal{D}$ over $\mathcal{X} \times \mathcal{Y}$,
prediction model $f_\theta: \mathbb{R}^D \to \mathbb{R}$ parameterized by $\theta\in \Theta \subset \mathbb{R}^M$,
and the loss function $l: \mathbb{R}\times \mathbb{R}\to \mathbb{R}$.

The loss function $L$ is defined by
\begin{equation}
L(\theta) := \mathbb{E}_{(x, y)\sim \mathcal{D}}\left[ l(f_\theta(x), y) \right]
\end{equation}

